ğ’° = Set
data â„• : ğ’° where
  zero : â„•
  suc  : â„• â†’ â„•
{-# BUILTIN NATURAL â„• #-}
bigNumber : â„•
bigNumber = 123456789  -- instead of suc (suc ( ... (suc ..)..
recâ„•
  : (C : ğ’°)
  â†’ C
  â†’ (â„• â†’ C â†’ C)
  -------------
  â†’ â„• â†’ C
recâ„• C câ‚€ câ‚› zero    = câ‚€
recâ„• C câ‚€ câ‚› (suc n) = câ‚› n (recâ„• C câ‚€ câ‚› n)
add : â„• â†’ â„• â†’ â„•
add = recâ„• (â„• â†’ â„•) (Î» m â†’ m) (Î» n g m â†’ suc (g m))

_+_ = add
infix 6 _+_
addâ‚‚ : â„• â†’ â„• â†’ â„•
addâ‚‚ zero    m = m
addâ‚‚ (suc n) m = suc (addâ‚‚ n m)
double : â„• â†’ â„•
double = recâ„• â„• 0 (Î» n y â†’ suc (suc y))
doubleâ‚‚ : â„• â†’ â„•
doubleâ‚‚ zero = zero
doubleâ‚‚ n    = suc (suc n)
open import Relation.Binary.PropositionalEquality using (refl; _â‰¡_; sym)

2+5 : add 2 5 â‰¡ 7
2+5 = refl

25+25 : add 25 25 â‰¡ 50
25+25 = refl
_*_ : â„• â†’ â„• â†’ â„•
_*_ = recâ„• (â„• â†’ â„•) (Î» m â†’ zero) (Î» n g m â†’ add m (g m))
infix 7 _*_
mâ‚ : 2 * 0 â‰¡ 0
mâ‚ = refl

mâ‚‚ : 2 * 3 â‰¡ 6
mâ‚‚ = refl

mâ‚ƒ : 10 * 3 â‰¡ 30
mâ‚ƒ = refl
indâ„•
  : âˆ€ {C : â„• â†’ ğ’°}
  â†’ C zero
  â†’ (âˆ€ (n : â„•) â†’ C n â†’ C (suc n))
  -------------------
  â†’ âˆ€ (n : â„•) â†’ C n
indâ„• câ‚€ câ‚› zero    = câ‚€
indâ„• câ‚€ câ‚› (suc n) = câ‚› n (indâ„• câ‚€ câ‚› n)
suc-cong
  : âˆ€ {n m : â„•}
  -----------------------
  â†’ n â‰¡ m â†’ suc n â‰¡ suc m

suc-cong refl = refl
addâ‰¡addâ‚‚
  : âˆ€ (n m : â„•)
  --------------------
  â†’ add n m â‰¡ addâ‚‚ n m

addâ‰¡addâ‚‚ zero    m = refl
addâ‰¡addâ‚‚ (suc n) m = suc-cong (addâ‰¡addâ‚‚ n m)
assoc
  : (i j k : â„•)
  ---------------------------
  â†’ i + (j + k) â‰¡ (i + j) + k
assocâ‚€
  : âˆ€ (j k : â„•)
  ---------------------------
  â†’ 0 + (j + k) â‰¡ (0 + j) + k

assocâ‚€ j k = refl
assocâ‚
  : âˆ€ (i : â„•)
  â†’ ((j k : â„•) â†’ i + (j + k) â‰¡ (i + j) + k)
  ---------------------------------------------------
  â†’ (j k : â„•) â†’ (suc i) + (j + k) â‰¡ ((suc i) + j) + k

assocâ‚ i p jâ‚ kâ‚ = suc-cong (p jâ‚ kâ‚)
assoc = indâ„• assocâ‚€ assocâ‚
+-commâ‚€
  : âˆ€ (m : â„•)
  ---------------
  â†’ 0 + m â‰¡ m + 0

+-commâ‚€ = indâ„• refl (Î» n indHyp â†’ suc-cong indHyp)
+-identity
  : âˆ€ (n : â„•)
  --------------
  â†’ n + zero â‰¡ n

+-identity = indâ„• refl (Î» n indHyp â†’ suc-cong indHyp)
+-suc
  : âˆ€ m n
  -------------------------
  â†’ m + suc n â‰¡ suc (m + n)

+-suc zero    n = refl
+-suc (suc m) n = suc-cong (+-suc m n)
trans
  : âˆ€ {m n p : â„•}
  â†’ m â‰¡ n â†’ n â‰¡ p
  ---------------
  â†’ m â‰¡ p

trans refl refl = refl
â‰¡sym
  : âˆ€ {m n p : â„•}
  â†’ m â‰¡ n â†’ n â‰¡ m

â‰¡sym refl = refl
+-comm
  : âˆ€ (m n : â„•)
  ---------------
  â†’ m + n â‰¡ n + m

+-comm =
  indâ„•
    sproofâ‚
    sproofâ‚‚
  where
    sproofâ‚
      : âˆ€ (n : â„•)
      ----------------
      â†’ n â‰¡ (n + zero)

    sproofâ‚ = indâ„• refl (Î» n nâ‰¡n+zero â†’ suc-cong nâ‰¡n+zero)

    sproofâ‚‚
      : âˆ€ (n : â„•)
      â†’ ((m : â„•) â†’ (n + m) â‰¡ (m + n))
      ---------------------------------------
      â†’ ((m : â„•) â†’ suc (n + m) â‰¡ (m + suc n))

    sproofâ‚‚ n hypâ‚ =
      indâ„•
        (suc-cong
          (hypâ‚ zero) )
        (Î» m hypâ‚‚ â†’
            suc-cong
              (trans
                  (hypâ‚ (suc m))
              (trans
                  (suc-cong
                      (sym (hypâ‚ m)))
                  hypâ‚‚)))
0+nâ‰¡n
  : âˆ€ (n : â„•)
  -----------
  â†’ 0 + n â‰¡ n

0+nâ‰¡n = indâ„• refl (Î» n p â†’ suc-cong p)
pâ‚‚
  : âˆ€ (n : â„•)
  -----------------------------------------
  â†’ double (n + 1) â‰¡ (suc (suc (double n)))

pâ‚‚ = indâ„• refl (Î» n indHyp â†’ suc-cong (suc-cong indHyp))
n+0â‰¡n
  : âˆ€ (n : â„•)
  -----------
  â†’ n + 0 â‰¡ n

n+0â‰¡n = indâ„• refl (Î» n indHyp â†’ suc-cong indHyp)
n+0â‰¡nâ‚‚
  : âˆ€ (n : â„•)
  -----------
  â†’ n + 0 â‰¡ n

n+0â‰¡nâ‚‚ zero    = refl
n+0â‰¡nâ‚‚ (suc n) = suc-cong (n+0â‰¡nâ‚‚ n)
module â„•-transInd (P : â„• â†’ ğ’°) where

  data _<_ : â„• â†’ â„• â†’ ğ’° where
    z<s : âˆ€ {n : â„•}   â†’ zero < suc n
    s<s : âˆ€ {m n : â„•} â†’ m < n â†’ suc m < suc n

  data _âŠ_ : ğ’° â†’ ğ’° â†’ ğ’° where
    injâ‚ : âˆ€ {A B : ğ’°} â†’ A â†’ A âŠ B
    injâ‚‚ : âˆ€ {A B : ğ’°} â†’ B â†’ A âŠ B

  âŠ-elim
    : âˆ€ {A B C : ğ’°}
    â†’ (A â†’ C)
    â†’ (B â†’ C)
    -------------
    â†’ (A âŠ B â†’ C)

  âŠ-elim f g (injâ‚ x) = f x
  âŠ-elim f g (injâ‚‚ y) = g y

  subst : {k n : â„•} â†’ k â‰¡ n â†’ P k â†’ P n
  subst refl pk = pk

  split-k<sucn
    : âˆ€ {k : â„•} {n : â„•}
    â†’ k < suc n
    -------------------
    â†’ (k < n) âŠ (k â‰¡ n)

  split-k<sucn {zero}  {zero}  k<sucn = injâ‚‚ refl
  split-k<sucn {zero}  {suc n} k<sucn = injâ‚ z<s
  split-k<sucn {suc k} {zero}  (s<s ())
  split-k<sucn {suc k} {suc n} (s<s k<sucn) =
    âŠ-elim
      (Î» k<n â†’ injâ‚ (s<s k<n))
      (Î» kâ‰¡n â†’ injâ‚‚ (suc-cong kâ‰¡n))
      (split-k<sucn k<sucn)
-- proof:
  indâ„•â‡’transFindâ„•
    : (hyp : (n : â„•) â†’ ((k : â„•) â†’ (k < n) â†’ P k) â†’ P n)
    â†’ ((n : â„•) â†’ P n)

  indâ„•â‡’transFindâ„• hyp zero    = hyp zero (Î» k â†’ Î» ())
  indâ„•â‡’transFindâ„• hyp (suc n) = hyp (suc n) (G (suc n))
    where
      G : âˆ€ (n : â„•) â†’ ((k : â„•) â†’ (k < n) â†’ P k)
      G zero    k () -- impossible case
      G (suc n) k k<n+1 =
        âŠ-elim
          -- 1. when k < n
          (Î» k<n â†’ G n k k<n)
          -- 2. when k â‰¡ n
          (Î» kâ‰¡n â†’ subst (sym kâ‰¡n) (hyp n (G n)))
          -- eliminiting two cases: (k < n) âŠ (k â‰¡ n)
          (split-k<sucn k<n+1)
