---
layout: "post"
title: "Solving some exercises of HoTT's book"
date: "2018-04-08"
categories: type-theory
toc: true
---

This is a self-contained version of some solutions for HoTT-Book's exercises.
The idea is to unpackage all as long as possible to get a better understanding.
Many changes can appear running this experiment. The solutions are
type-checked as a whole using Agda v2.5.3.

## Requirements

-------------------------------------------------------------------------------

Agda has a pragma to work with HoTT:

\begin{code}
{-# OPTIONS --without-K #-}
\end{code}

-------------------------------------------------------------------------------

Equality type defintion also called Identity type:

\begin{code}
infix 4 _â‰¡_
data _â‰¡_ {a} {A : Set a} (x : A) : A â†’ Set a where
  refl : x â‰¡ x
\end{code}

Some functions to work with this type:

\begin{code}
sym : âˆ€ {i} {A : Set i} {x y : A}
    â†’ x â‰¡ y â†’ y â‰¡ x
sym refl = refl

_Â·_ : âˆ€ {i}{X : Set i}{x y z : X}
    â†’ x â‰¡ y â†’ y â‰¡ z â†’ x â‰¡ z
refl Â· p = p
infixl 9 _Â·_

ap : âˆ€ {i j}{A : Set i}{B : Set j}{x y : A}
   â†’ (f : A â†’ B) â†’ x â‰¡ y â†’ f x â‰¡ f y
ap f refl = refl

apâ‚‚ : âˆ€ {i j} {A B : Set i}{C : Set j}
      {xâ‚€ xâ‚ : A}{yâ‚€ yâ‚ : B}
    â†’ (f : A â†’ B â†’ C) â†’ (xâ‚€ â‰¡ xâ‚) â†’ (yâ‚€ â‰¡ yâ‚)
    â†’ f xâ‚€ yâ‚€ â‰¡ f xâ‚ yâ‚
apâ‚‚ f refl refl = refl

subst : âˆ€ {i j} {A : Set i}{x y : A}
      â†’ (B : A â†’ Set j) â†’ x â‰¡ y
      â†’ B x â†’ B y
subst B refl = (Î» z â†’ z)

\end{code}

Path induction:

\begin{code}
J' : âˆ€ {i j}{X : Set i}{x : X}
   â†’ (P : (y : X) â†’ x â‰¡ y â†’ Set j)
   â†’ P x refl
   â†’ (y : X)
   â†’ (p : x â‰¡ y)
   â†’ P y p
J' P u y refl = u

J : âˆ€ {i j}{X : Set i}
  â†’ (P : (x y : X) â†’ x â‰¡ y â†’ Set j)
  â†’ ((x : X) â†’ P x x refl)
  â†’ (x y : X)
  â†’ (p : x â‰¡ y)
  â†’ P x y p
J P u x y p = J' (P x) (u x) y p
\end{code}

-----------------------------------------------------------------------------

## Chapter 1

### Exercise 1.1

<div class="exercise">
Given functions $$f : A \to B$$ and $$g:B\to C$$, define
their composite $$ g\circ f:A\to C$$.
Show that we have $$h \circ (g\circ f) \equiv (h\circ g)\circ f$$.
</div>

We define the composition operation in Agda as follows.

\begin{code}
_âˆ˜_ : âˆ€ {i j k} {A : Set i}{B : Set j}{C : Set k}
    â†’ (B â†’ C)
    â†’ (A â†’ B)
    â†’ A â†’ C
g âˆ˜ f = Î» x â†’ g (f x)
\end{code}

Then, the `âˆ˜-assoc` shows us that associativity of this composition holds.

\begin{code}
âˆ˜-assoc : âˆ€ {i j k l} {A : Set i}{B : Set j}{C : Set k}{D : Set l}
        â†’ (h : C â†’ D)(g : B â†’ C)(f : A â†’ B)
        â†’ h âˆ˜ (g âˆ˜ f) â‰¡ (h âˆ˜ g) âˆ˜ f
âˆ˜-assoc f g h = refl
\end{code}

### Exercise 1.2

<div class="exercise">
Derive the recursion principle for products $$\mathsf{rec}_{A\times B}$$
using only the projections, and verify that the definitional equalities
are valid. Do the same for $$\Sigma$$-types.
</div>

To solve this problem we need to know:

  - The recursion principle for Î£-types:

    <p class="equation">
    $$ \mathsf{rec}_{ A \times B}
      : \prod\limits_{C : \mathcal{U}} (A \to B \to C) â†’ A \times B \to C.
    $$
    </p>

  - The recursion principle for Î£-types:

    <p class="equation">
    $$ \mathsf{rec}_{\sum\limits_{(x : A) } B(x)}
      : \prod\limits_{(C : U)} (\Pi_{(x : A)} B(x) \rightarrow C) \rightarrow
        \sum_{(x : A)} B(x) \rightarrow C
    $$
    </p>

<div class="proof" id="proof-1.2">
Proof.<br/>
For products:<br/>
If we have the projections,
$$\mathsf{proj}_1 : A \times B \to \mathsf{A}$$ and $$\mathsf{proj}_2 : A \times B \to \mathsf{B}$$,
then $$\mathsf{rec}_2$$ is another inhabitant where

<p class="equation">
$$
\begin{align*}
&\mathsf{rec}_1 : \prod\limits_{C : \mathcal{U}} (A \to B \to C) \to A \times B \to C\\
&\mathsf{rec}_1~C~g~c~:\equiv~g~(\mathsf{proj}_1 c,~\mathsf{proj}_2 c).
\end{align*}
$$
</p>
By reflexivity, we prove the equality between $$\mathsf{rec}_{ A \times B}$$ and $$\mathsf{rec}_1$$.
<br/>
<br/>
For sums:<br/>
The projections are $$\mathsf{proj}_1 : \sum_{x : A}  Bx \to \mathsf{A}$$ and
$$\mathsf{proj}_2 :  \prod_{(p : \sum_{x : A}  Bx)} \to \mathsf{B} (\mathsf{proj}_1 p)$$.<br/>
By using these projections, we got another recursor defined as follows:
<p class="equation">
$$
\begin{aling*}
&\mathsf{rec}_2 : \prod\limits_{C : \mathcal{U}}  (\prod_{x : A} Bx \to C) \to \sum\limits_{x : A} B x \to C\\
&\mathsf{rec}_2~C~g~c~=~g~(\mathsf{proj}_1 c)~(\mathsf{proj}_2 c)
\end{align*}
$$
</p>

By reflexivity, we prove the equality between $$\mathsf{rec}_{\sum\limits_{(x : A) } B(x)}$$ and $$\mathsf{rec}_2$$.
</div>

-------------------------------------------------------------------------------

In Agda.<br>

Let's add some machinery to handle levels of the universe needed for
the following exercises including this one:

\begin{code}
open import Agda.Primitive public
  using (Level; _âŠ”_; lzero; lsuc)
\end{code}

Î£-type (sigma type) definition (see the definition without projections
[here](https://github.com/jonaprieto/hott-book/blob/master/other/prelim.agda#L20)):

\begin{code}
module Î£-Defâ‚ where

  record Î£ {a b} (A : Set a) (B : A â†’ Set b) : Set (a âŠ” b) where
    constructor _,_
    field
      projâ‚ : A
      projâ‚‚ : B projâ‚

  open Î£ public
-- _,_ : (projâ‚ : A) â†’ B projâ‚ â†’ Î£ A B.
\end{code}

Its recursor with a function $$g : \prod_{(x : A)} B(x)\rightarrow C$$
that we provide.

\begin{code}
module Î£-Recâ‚ {i j k}{A : Set i}{B : A â†’ Set j}{C : Set k}
             (g : (x : A) â†’ B x â†’ C) where

  open Î£-Defâ‚ using (Î£ ; projâ‚; projâ‚‚; _,_ )

  rec : Î£ A B â†’ C
  rec p = g (projâ‚ p) (projâ‚‚ p)

  rec-Î² : (x : A)(y : B x) â†’ rec (x , y) â‰¡ g x y
  rec-Î² x y = refl
\end{code}

-------------------------------------------------------------------------------

On the other hand, the product type is just a particular case of the sigma type
when the codomain is not dependent, as we can see next by omitting the argument
in `(Î» _ â†’ B)`.

\begin{code}
module Ã—-Defâ‚ where
  open Î£-Defâ‚ public

  _Ã—_ : {l k : Level} (A : Set l) (B : Set k) â†’ Set (l âŠ” k)
  A Ã— B = Î£ A (Î» _ â†’ B)
\end{code}

Its recursor with a function $$g : A \rightarrow B \rightarrow C$$ that we provide.

\begin{code}
module Ã—-Recâ‚ {i j k}{A : Set i}{B : Set j}{C : Set k} (g : A â†’ B â†’ C) where

  open Ã—-Defâ‚ using (_Ã—_; projâ‚; projâ‚‚; _,_)

  rec : A Ã— B â†’ C
  rec p = g (projâ‚ p) (projâ‚‚ p)

  rec-Î² : (x : A)(y : B) â†’ rec (x , y) â‰¡ g x y
  rec-Î² x y = refl
\end{code}

### Exercise 1.3

<p class="exercise">
Derive the induction principle for products $$\mathsf{ind}_{A\times B}$$,
using only the projections and the propositional uniqueness principle
$$\mathsf{uniq}_{A\times B}$$.
Verify that the definitional equalities are valid.
</p>

To solve this problem, recall the uniqueness principle (Pp. 29. HoTT-Book)

- The **propositional uniqueness principle** says that
every element of $$A\times B$$ is equal to a pair.

<p class="equation">
  $$ \mathsf{uniq}_{A\times B}
     : \prod_{(x : A \times B)} ((\mathsf{proj}_{1}(x) , \mathsf{proj}_{2}(x))
       \equiv_{A\times B} x).
  $$
</p>

Product type definition using `data`:

\begin{code}
-- this would be trivial in agda due to definitional Î· for records
-- so Capriotti defined a product type without Î·:
module Ã—-Defâ‚‚ where

  data _Ã—_ {i j}(A : Set i)(B : Set j) : Set (i âŠ” j) where
    _,_ : A â†’ B â†’ A Ã— B

  projâ‚ : âˆ€ {i j}{A : Set i}{B : Set j}
        â†’ A Ã— B â†’ A
  projâ‚ (a , b) = a

  projâ‚‚ : âˆ€ {i j}{A : Set i}{B : Set j}
        â†’ A Ã— B â†’ B
  projâ‚‚ (a , b) = b
\end{code}

Projections and $$\mathsf{uniq}_{A\times B}$$:

\begin{code}
module Ã—-Funâ‚‚ {i j}{A : Set i}{B : Set j} where
  open Ã—-Defâ‚‚ using ( _Ã—_;_,_; projâ‚; projâ‚‚)

  -- propositional uniqueness principle:
  uppt : (x : A Ã— B) â†’ (projâ‚ x , projâ‚‚ x) â‰¡ x
  uppt (a , b) = refl

  -- (ap functions): (a)ction over a (p)ath
  ap-projâ‚ : {A B : Set}{x y : A Ã— B}
           â†’ (x â‰¡ y) â†’ projâ‚ x â‰¡ projâ‚ y
  ap-projâ‚ refl = refl

  ap-projâ‚‚ : {A B : Set}{x y : A Ã— B}
           â†’ (x â‰¡ y) â†’ projâ‚‚ x â‰¡ projâ‚‚ y
  ap-projâ‚‚ refl = refl

  pair= : âˆ€ {A B : Set} {x w : A} {y z : B}
        â†’ x â‰¡ w â†’ y â‰¡ z â†’ (x , y) â‰¡ (w , z)
  pair= refl refl = refl
\end{code}

The induction principle for the product type:

<p class="equation">
$$\mathsf{ind}_{A\times B} : \prod\limits_{C : A \times B \to \mathcal{U}}
  \left( \prod\limits_{x:A}\ \prod\limits_{y:B}\ \,C( (x,y) ) \right)
  \to \prod\limits_{x:A \times B}\ \,C(x)
$$
</p>

\begin{code}
module Ã—-Indâ‚‚ {i j}{A : Set i}{B : Set j} where
  open Ã—-Defâ‚‚ using (_Ã—_; _,_;projâ‚;projâ‚‚)
  open Ã—-Funâ‚‚ using (uppt)

  ind : âˆ€ {k}(C : A Ã— B â†’ Set k)
        â†’ ((x : A)(y : B) â†’ C (x , y))
        â†’ (x : A Ã— B) â†’ C x
  ind C g x = subst C (uppt x) (g (projâ‚ x) (projâ‚‚ x))

  ind-Î² : âˆ€ {k} (C : A Ã— B â†’ Set k)
          â†’ (g : (x : A)(y : B) â†’ C (x , y))
          â†’ (x : A)(y : B)
          â†’ ind C g (x , y) â‰¡ g x y
  ind-Î² C g x y = refl
\end{code}

<p class="exercise">
Generalize $$\mathsf{uniq}_{A\times B}$$ to Î£-types, and do the same for
$$\Sigma$$-types, i.e. show induction and verify the definitional equality
is valid.
</p>

Î£-type definition using `data`:

\begin{code}
module Î£-Defâ‚‚ where

  data Î£ {i j}(A : Set i)(B : A â†’ Set j) : Set (i âŠ” j) where
    _,_ : (x : A) â†’ B x â†’ Î£ A B
\end{code}

Projections and uniqueness propositional principle:

\begin{code}
module Î£-Funâ‚‚ {i j } {A : Set i}{B : A â†’ Set j} where
  open Î£-Defâ‚‚ using (Î£; _,_ )

  projâ‚ : Î£ A B â†’ A
  projâ‚ (a , b) = a

  projâ‚‚ : (x : Î£ A B) â†’ B (projâ‚ x)
  projâ‚‚ (a , b) = b

  uppt : (x : Î£ A B) â†’ (projâ‚ x , projâ‚‚ x) â‰¡ x
  uppt (a , b) = refl
\end{code}

Its induction principle:

\begin{code}
module Î£-Indâ‚‚ {i j}{A : Set i}{B : A â†’ Set j} where
  open Î£-Defâ‚‚ public
  open Î£-Funâ‚‚ public

  ind : (C : Î£ A B â†’ Set (i âŠ” j))
        â†’ ((x : A)(y : B x) â†’ C (x , y))
        â†’ (x : Î£ A B) â†’ C x
  ind C g (a , b) = g a b

  ind-Î² : (C : Î£ A B â†’ Set (i âŠ” j))
          â†’ (g : (x : A)(y : B x) â†’ C (x , y))
          â†’ (x : A) (y : B x)
          â†’ (ind C g (x , y)) â‰¡ g x y
  ind-Î² C g x y = refl
\end{code}

### Exercise 1.4

<div class="exercise">
Assuming as given only the <em>iterator</em> for natural numbers
<p class="equation">
$$\mathsf{ite} : \prod\limits_{C:\mathcal{U}} C \to (C \to C) \to \mathbb{N} \to C $$
</p>
with the defining equations
<p class="equation">
$$
\begin{align*}
\mathsf{ite}(C,c_0,c_s,0)               &\equiv c_0, \\
\mathsf{ite}(C,c_0,c_s,\mathsf{suc}(n)) &\equiv c_s(\mathsf{ite}(C,c_0,c_s,n)),
\end{align*}
$$
</p>
derive a function having the type of the recursor $$\mathsf{rec}$$.
Show that the defining equations of the recursor hold propositionally for this
function, using the induction principle for $$\mathbb{N}$$.
</div>

To solve this problem, let us define the recursor and also the induction principle
for natural numbers. (See more details about these functions in
[Induction on Natural Numbers]({% post_url 2018-02-12-induction-on-natural-numbers %})).

\begin{code}
module â„•-Def where

  data â„• : Set where
    zero : â„•
    suc  : â„• â†’ â„•

module â„•-Rec where
  open â„•-Def
  rec : âˆ€ (C : Set) â†’ C â†’ (â„• â†’ C â†’ C) â†’ â„• â†’ C
  rec C câ‚€ câ‚› zero    = câ‚€
  rec C câ‚€ câ‚› (suc n) = câ‚› n (rec C câ‚€ câ‚› n)

module â„•-Ind where
  open â„•-Def
  ind : âˆ€ (C : â„• â†’ Set)
       â†’ (C zero)
       â†’ (âˆ€ (n : â„•) â†’ C n â†’ C (suc n))
       â†’ (âˆ€ (n : â„•) â†’ C n)
  ind C câ‚€ câ‚› zero    = câ‚€
  ind C câ‚€ câ‚› (suc n) = câ‚› n (ind C câ‚€ câ‚› n)
\end{code}

Now, we define the iterator following the equations above:

\begin{code}
module â„•-Fun where
  open â„•-Def using (â„•; zero; suc)
  open â„•-Rec using (rec)

  ite : âˆ€ (C : Set) â†’ C â†’ (C â†’ C) â†’ â„• â†’ C
  ite C câ‚€ câ‚› zero    = câ‚€
  ite C câ‚€ câ‚› (suc n) = câ‚› (ite C câ‚€ câ‚› n)
\end{code}

Then, we now can define the recursor using this `ite` by iterating over the type
`â„• Ã— C` (*reloading recursion*?).


\begin{code}
-- recursor
  open Ã—-Defâ‚‚ using (_Ã—_; projâ‚; projâ‚‚; _,_)

  recâ‚‚ : âˆ€ (C : Set) â†’ C â†’ (â„• â†’ C â†’ C) â†’ â„• â†’ (â„• Ã— C)
  recâ‚‚ C câ‚€ câ‚› n =
      (ite (â„• Ã— C)
           (zero , câ‚€)
           (Î» (p : â„• Ã— C) â†’ (suc (projâ‚ p) , câ‚› (projâ‚ p) (projâ‚‚ p)))
           n)
\end{code}

Now, we need to establish the propositional equality between these two
definitions of recursor, i.e, between `rec` and `recâ‚‚`. Let's use
induction to prove that.

\begin{code}
module ex1-4 where

  open â„•-Def using (â„•; zero; suc)
  open â„•-Rec using (rec)
  open â„•-Ind using (ind)
  open â„•-Fun using (ite; recâ‚‚)

  open Ã—-Defâ‚‚ using (_Ã—_; projâ‚; projâ‚‚; _,_)
  open Ã—-Funâ‚‚

  proof : (C : Set)(câ‚€ : C)(câ‚› : â„• â†’ C â†’ C)
        â†’ âˆ€ (n : â„•) â†’ recâ‚‚ C câ‚€ câ‚› n â‰¡ (n , rec C câ‚€ câ‚› n)

  proof C câ‚€ câ‚› zero    = refl
  proof C câ‚€ câ‚› (suc n) = pair= {A = â„•}{B = C} (ap suc v) (apâ‚‚ câ‚› v u)
    where
      v : projâ‚ {A = â„•}{B = C}
        (ite
            (â„• Ã— C)
            (zero , câ‚€)
            (Î» p â†’ suc (projâ‚ p) , câ‚› (projâ‚ p) (projâ‚‚ p)) n)
         â‰¡ n
      v = (ap-projâ‚ {A = â„•}{B = C} (proof C câ‚€ câ‚› n))

      u : projâ‚‚ {A = â„•}{B = C} (recâ‚‚ C câ‚€ câ‚› n) â‰¡ rec C câ‚€ câ‚› n
      u = ap-projâ‚‚  {A = â„•}{B = C} (proof C câ‚€ câ‚› n)
\end{code}


### Exercise 1.5

<div class="exercise">

Show that if we define

  $$A+B :\equiv \sum\limits_{(x : \mathbbbold{2})} \mathsf{rec}_{\mathbbbold{2}} (\mathcal{U}, A , B, x),$$

then we can give a definition of $$\ind\limits_{A + B}$$ for which the
definitional equalities holds.

</div>

To solve this problem, let us introduce the $$\mathcal{2}$$ type, that is, the
type with two constructors also called **Bool**. The constructors are also called
false and true respectively.

\begin{code}
module ğŸš-Defâ‚ where

  data ğŸš : Set where
    ğŸ˜ : ğŸš
    ğŸ™ : ğŸš
\end{code}


With the recursor:

\begin{code}
module ğŸš-Recâ‚ where

  open ğŸš-Defâ‚  using (ğŸ˜;ğŸ™;ğŸš)

  rec : âˆ€ {i} {C : Set i} (a : C) (b : C ) â†’ ğŸš â†’ C
  rec a b ğŸ˜ = a
  rec a b ğŸ™ = b
  -- rec is the same if_then_else
\end{code}

and its induction principle:

\begin{code}
module ğŸš-Indâ‚ where

  open ğŸš-Defâ‚ using (ğŸ˜;ğŸ™;ğŸš)

  ind : âˆ€ {i} {C : ğŸš â†’ Set i} â†’ C ğŸ˜ â†’ C ğŸ™ â†’ (c : ğŸš) â†’ C c
  ind câ‚€ câ‚ ğŸ˜ = câ‚€
  ind câ‚€ câ‚ ğŸ™ = câ‚
\end{code}


The we define the **coproduct** $$A+B$$ as follows:

\begin{code}
module +-Defâ‚ where

  open Î£-Defâ‚ using (Î£;_,_;projâ‚; projâ‚‚) public

  open ğŸš-Defâ‚ using (ğŸ˜;ğŸ™;ğŸš)
  open ğŸš-Recâ‚ using (rec)

  _+_ : âˆ€ {i} (A B : Set i) â†’ Set _
  A + B = Î£ ğŸš (rec A B) -- if it's ğŸ˜ return A otherwise returns B

  -- the tradional constructors
  inl : âˆ€ {i}{A B : Set i} â†’ A â†’ A + B
  inl a = (ğŸ˜ , a)

  inr : âˆ€ {i}{A B : Set i} â†’ B â†’ A + B
  inr b = (ğŸ™ , b)
\end{code}


Now, let's try to define the recursor for this coproduct, and later,
we'll try the dependent version of it to complete the exercise.

\begin{code}
module +-Recâ‚ where

  open +-Defâ‚ using (_+_; inl;inr;_,_)
  open ğŸš-Defâ‚ using (ğŸ˜;ğŸ™;ğŸš)

  rec : âˆ€ {i j} {A B : Set i} {C : Set j}
      â†’ (A â†’ C)
      â†’ (B â†’ C)
      â†’ A + B â†’ C
  rec f g (ğŸ˜ , a) = f a
  rec f g (ğŸ™ , b) = g b
\end{code}


Notice how the recursor of the coproduct matches with the elimination
rule of the disjunction conective also called *case analysis*. That's follows from the
[**propositions-as-types**](https://ncatlab.org/nlab/show/propositions+as+types).

![path](/assets/latexit-images/disj-elimination.png)

Finally, the induction principle for the coproduct:

\begin{code}
module +-Indâ‚ where

  open +-Defâ‚ using (_+_; inl;inr; _,_)
  open ğŸš-Defâ‚ using (ğŸ˜;ğŸ™;ğŸš)

  ind : âˆ€ {i j} {A B : Set i} {C : A + B â†’ Set j}
      â†’ ((a : A) â†’ C (inl a))
      â†’ ((b : B) â†’ C (inr b))
      â†’ (p : A + B) â†’ C p
  ind f g (ğŸ˜ , a) = f a -- TODO any reason to not use this definition?
  ind f g (ğŸ™ , b) = g b

  ind-Î²â‚ : âˆ€ {i j} {A B : Set i} {C : A + B â†’ Set j}
      â†’ (f : (a : A) â†’ C (inl a))
      â†’ (g : (b : B) â†’ C (inr b))
      â†’ (x : A) â†’ ind {C = C} f g (inl x) â‰¡ f x
  ind-Î²â‚ f g x = refl

  ind-Î²â‚‚ : âˆ€ {i j} {A B : Set i} {C : A + B â†’ Set j}
      â†’ (f : (a : A) â†’ C (inl a))
      â†’ (g : (b : B) â†’ C (inr b))
      â†’ (x : B) â†’ ind {C = C} f g (inr x) â‰¡ g x
  ind-Î²â‚‚ f g x = refl
\end{code}

## Chapter 2



## Chapter 3

To solve the following exercises, let us recall a few things:

- The *set* definition in HoTT:

A type $$A$$ is a **set** if for all $$x, y : A$$ and
all $$p, q : x \equiv y$$, we have $$ p \equiv q$$. In a proposition
we have

$$
\mathsf{isSet}(A) :\equiv \prod\limits_{(x,y : A)}\prod\limits_{(p,q : x \equiv y)} (p \equiv q).
$$

- The type for equivalence from $$A$$ to $$B$$

$$
  (A \simeq B) :\equiv \sum\limits_{f : A \to B} \mathsf{isequiv}(f),
$$

where

$$
\mathsf{isequiv(f)} :\equiv
  \left (\sum\limits_{g : B \to A} (f \circ g \sim \mathsf{id}_{B})\right) \times
  \left (\sum\limits_{h : B \to A} (h \circ f \sim \mathsf{id}_{A})\right)
$$

- The homotopy concept:

Let $$f , g : \prod\limits_{(x:A)} P(x)$$ be two sections of a
type family $$P : A \to \mathcal{U}$$. A **homotopy** from $$f$$ to $$g$$
is a dependent function of type

$$
(f \sim g) :\equiv \prod\limits_{x : A} (f(x) \equiv g(x)).
$$

### Exercise 3.1

<div class="exercise">
Prove that if $$A\simeq B$$ and $$A$$ is a set, then so is $$B$$.
</div>


<div class="proof" id="proof-3.1">
Proof.<br/>
Let be $$x,y : B$$ and $$p : x \equiv_{B} y$$ and $$q : x \equiv_{B} y$$.
We need to prove $$ p \equiv q$$.<br/>
Since $$A\simeq B$$ then there is a function $$f : A \to B$$ and some
$$g : B \to A$$ such that $$f \circ g \sim id_{B}$$.
Using this function $$g$$ over the path $$p$$ we get
$$\mathsf{ap}_{g} p : g x \equiv_{A} g y$$.
We do the same but this time over the path $$q$$, that is,
$$\mathsf{ap}_{g} q : g x \equiv_{A} g y$$.
Because of $$A$$ is a set, we have a new path called
$$m :\mathsf{ap}_{g} p \equiv_{gx \equiv_{A} gy} \mathsf{ap}_{g} q$$. <br/>

Now, an action over this path $$m$$
using the function $$\mathsf{ap}_{f} : x \equiv_{A} y \to f x \equiv_{B} f y$$
will give us

<p class="equation">
$$
\mathsf{ap}_{\mathsf{ap}_{f}} m :
(\mathsf{ap}_{f}) (\mathsf{ap}_{g} p) \equiv (\mathsf{ap}_{f})  (\mathsf{ap}_{g} q).
$$
</p>
By the lemmas in Chapter 2, we do the following reasoning:

<p class="equation">
$$
\begin{align*}
(\mathsf{ap}_{f}) (\mathsf{ap}_{g} p) \equiv (\mathsf{ap}_{f})  (\mathsf{ap}_{g} q) &=
  \mathsf{ap}_{f \circ g} p \equiv \mathsf{ap}_{f \circ g} q\\
  &=\mathsf{ap}_{\mathsf{id}_{B}} p \equiv \mathsf{ap}_{\mathsf{id}_{B}} q\\
  &= p \equiv q.
\end{align*}
$$<br/>
</p>
Then, we have the inhabitant, $$\mathsf{ap}_{\mathsf{ap}_{f}} m : p \equiv q$$.
</div>


In Agda:

\begin{code}
module sets where

  isSet : âˆ€ {i} (A : Set i) â†’ Set _
  isSet A = (x y : A) â†’ (p : x â‰¡ y) â†’ (q : x â‰¡ y) â†’ p â‰¡ q
  -- TODO
\end{code}

### Exercise 3.2

<div class="exercise">
Prove that if $$A$$ and $$B$$ are sets, then so is $$A+B$$.
</div>

To solve this exercise, we should take a look of some results from Chapter 2,
Section 2.12.

<div class="proof" id="proof-3.2">
Proof.<br/>

Let be $$x, y : A + B$$, and paths $$p : x \equiv y$$, $$q : x \equiv
y$$. Let's get a path $$p \equiv q$$.  We proceed by case analysis. If
$$x :\equiv \mathsf{inl} a$$ and $$y :\equiv \mathsf{inl} b$$, for
some $$a, b : A$$ then $$\mathsf{ap}_{\mathsf{inl}^{-1}} p : a
\equiv_{A} b$$ and $$\mathsf{ap}_{\mathsf{inl}^{-1}} q : a \equiv_{A}
b$$.

Since $$A$$ is a set, there is a path between these last two terms,
this is, $$m : \mathsf{ap}_{\mathsf{inl}^{-1}} p \equiv
\mathsf{ap}_{\mathsf{inl}^{-1}} q$$.  Now, an action over this path
$$m$$ using the $$\mathsf{inl}$$ function give us:
$$\mathsf{ap}_{\mathsf{inl}} m : \mathsf{ap}_{\mathsf{inl}}
(\mathsf{ap}_{\mathsf{inl}^{-1}} p) \equiv \mathsf{ap}_{\mathsf{inl}}
(\mathsf{ap}_{\mathsf{inl}^{-1}} q)$$.<br/>

We conclude by Lemmas in Chapter 2, that $$\mathsf{ap}_{\mathsf{inl}}
m : p \equiv q$$ since $$\mathsf{ap}_{\mathsf{inl}}
(\mathsf{ap}_{\mathsf{inl}^{-1}} p) \equiv p$$.<br/> Following the
same reasoning, we prove the case $$x :\equiv \mathsf{inr} a$$ and $$y
:\equiv \mathsf{inr} b$$.  For the latest cases, $$x :\equiv
\mathsf{inl} a$$ and $$y :\equiv \mathsf{inr} b$$ and $$x :\equiv
\mathsf{inr} a$$ and $$y :\equiv \mathsf{inl} b$$, we use the
encode-decode method to derive a proof term for ğŸ˜ from
$$p$$ and $$q$$. Then, we may conclude anything we wish, that is, $$p
\equiv q$$.
</div>

In Agda.

\begin{code}
module ğŸ˜-Def where
  data ğŸ˜ : Set where

module ğŸ˜-Rec where
  open ğŸ˜-Def
  rec : {A : Set} â†’ ğŸ˜ â†’ A
  rec = Î» ()
\end{code}

\begin{code}
module +-Defâ‚‚ where

  data _+_ : Set â†’ Set â†’ Setâ‚ where
    inl : âˆ€ {B : Set} â†’ (A : Set) â†’ A + B
    inr : âˆ€ {A : Set} â†’ (B : Set) â†’ A + B

module +-Funâ‚‚ where

  open +-Defâ‚‚
  open ğŸ˜-Def
  open ğŸ˜-Rec

  code : {A B : Set}
       â†’ A + B â†’ Set _
  code {A}{B} (inl a) = a â‰¡ a
  code {A}{B} (inr b) = {!!}

module +-Recâ‚‚ where
  open +-Defâ‚‚

  rec : {A B : Set}
      â†’ (C : Set)
      â†’ (A â†’ C)
      â†’ (B â†’ C)
      â†’ A + B â†’ C
  rec C f g (inl A) = f {! a  !}
  rec C f g (inr B) = g {!   !}

module +-Indâ‚‚ where
  open +-Defâ‚‚

  -- ind : {A B : Set}
  --     â†’ (C : A + B â†’ Set)
  --     â†’ ((x : A) â†’ C (inl x))
  --     â†’ ((x : B) â†’ C (inr x))
  --     â†’ (x : A + B) â†’ C x
  -- ind C f g c x = {!   !}

-- module +-Funâ‚‚ where
\end{code}


\begin{code}
module ex3-2 where
  open +-Defâ‚‚
  open sets using (isSet)

  p : {A B : Set}
    â†’ isSet A â†’ isSet B â†’ isSet (A + B)
  p {.A} {B} setA setB (inl A) (inl .A) refl refl = refl
  p {A} {.B} setA setB (inr B) (inr .B) refl refl = refl
  p {.A} {.B} setA setB (inl A) (inr B) p q = {!   !}
  p {.A} {.B} setA setB (inr B) (inl A) p q = {!   !}
\end{code}

### Exercise 3.3

<div class="exercise">
Prove that if $$ A $$ is a set and $$B : A \to \mathcal{U}$$
is a type family such that $$B(x)$$ is a set for all
$$x : A$$, then $$\Sigma\limits_{(x:A)}\ B(x)$$ is a set.
</div>

### Exercise 3.4

<div class="exercise">
Show that $$A$$ is a mere proposition if and only
if $$A\to A$$ is contractible.
</div>

### References

{::options parse_block_html="true" /}
<div class="references">

  - {% reference hottbook %}

  - {% reference Grayson2017 %}

  - {% reference Wadler2015PT %}

  - [Capriotti's hott-exercises](https://github.com/pcapriotti/hott-exercises)

  - [Capriotti's agda-base](https://github.com/pcapriotti/agda-base/)
</div>
{::options parse_block_html="false" /}
